\documentclass[12pt]{article}
\usepackage{amsmath}
\usepackage{graphicx}
\usepackage{hyperref}
\usepackage[latin1]{inputenc}

\title{Financial Math}
\author{Samuel Du}
\date{01/05/2011}

\begin{document}
\maketitle

Welcome to my math book on Financial Math


Chapter 1: Forwards, Futures, and Swaps
\paragraph{Forward Prices}
\begin{itemize}
	\item Forwards on stock S(t)\\
	Base on no arbitrage arguments of using debt S(t) to buy and hold one share to sell at time T, we find:

 \begin{center} F(t) = ${e^{r(T-t)}}$ S(t) \end{center}
 
 Similarly,
 
 \item Forwards on stock paying dividend rate q
 
 \begin{center} F(t) = ${e^{(r-q)(T-t)}}$ S(t) \end{center}
 
 \item Forwards on foreign currency priced S(t) in domestic currency and paying foreign interest rate ${r_f}$
 	\begin{center} F(t) = ${e^{(r-r_f)(T-t)}}$ S(t) \end{center}
 	
 \item Problems with Forward Contracts \\
 	Counter party risk and liquidity risks
 \end{itemize}

\paragraph{Futures Prices}

 
\begin{itemize}
	\item Future prices and forward prices are identical if interest rate is deterministic
	\item 
  
\end{itemize}

\paragraph{Swaps}
\begin{itemize}
	\item Swap price is the linear combination of zero rates\\
	${C_i = \Delta T[L(T_{i-1}, T_i)-R]}$\\
	${L(T_{i-1}, T_i):= \frac{1-P(T_{i-1}, T_i)}{\Delta T P(T_{i-1}, T_i)}}$\\
	${C_i=\frac{1-P(T_{i-1}, T_i)}{P(T_{i-1}, T_i)}-(R\Delta T)}$\\
	in terms of present value then,\\
	${C_i(t)={\frac{1-P(T_{i-1}, T_i)}{P(T_{i-1}, T_i)} P(t, T_{i})}-(R\Delta T)P(t,T_i)}\\=[P(t, T_{i-1})- P(t, T_i)]-(R\Delta T) P(t, T_i)$\\
	=present value of float - present value of fixed
	\\
	\item An important thing to see there is that the present value of swap cash flows is a linear combination of discount factors, which are in turn completely determined by the current yield curve.\\
	
	Now, the value of the swap is:\\
	${S(t)=\sum_{i=1}^n C_i(t)=\sum_{i=1}^n [P(t, T_{i-1}-(1+R\Delta T ) P(t, T_i)]}$\\
	
		 ${S(t)=P(t, T_0)-R \Delta T \sum_{i=1}^{n} P(t, T_i) -P(t, T_n) }$ 
	\item setting swap price S(t) to 0 and derive the fixed swap rate R, we have the fixed swap rate,\\
	${R=\frac{P(0, T_0)-P(0, T_n)}{\Delta T \sum_{i=1}^n P(0, T_i)} }$ 
  
\end{itemize}



\end{document}
